### 2.1.

1.  $\beta_0$ is the predicted value when $x = 0$
2.  $\alpha_0$ is the predicted value when $x$ is equal to the mean of $x$ (that is, $\bar{x}$). The second form may allow a better interpretation of the constant, since $x = 0$ may be far from the values of $x$ used to fit the model.

### 2.2

$$\frac{\partial S}{\partial \beta_0} = 2 \Sigma_{i=1}^{n} w_i(y_i - \mu_i) = 0 \tag{1}$$ $$\frac{\partial S}{\partial \beta_1} = 2 \Sigma_{i=1}^{n} w_ix_i(y_i - \mu_i) \tag{2}= 0$$ From the above,

<!-- $$ -->
<!-- \begin{align*} -->
<!--   (1) \Leftrightarrow \frac{\partial S}{\partial \beta_0} &= 0 \\ -->
<!--   \Sigma_{i=1}^{n} w_i(y_i - \mu_i) &= 0 \\ -->
<!--   \Sigma_{i=1}^{n} w_i(y_i - \beta_0 - \beta_1 x_i) &= 0 \\ -->
<!--   \beta_0 \Sigma_{i=1}^{n} w_i &= \Sigma_{i=1}^{n} w_iy_i - \beta_1 \Sigma_{i=1}^{n} w_i x_i \\ -->
<!--   \beta_0 &= \frac{\Sigma_{i=1}^{n} w_iy_i}{\Sigma_{i=1}^{n} w_i} - \beta_1 \frac{\Sigma_{i=1}^{n} w_i x_i}{\Sigma_{i=1}^{n} w_i} \\ -->
<!--   \beta_0 &= \bar{y}_w - \beta_1 \bar{x}_w  -->
<!-- \end{align*} -->
<!-- $$ -->

$$
\begin{align*}
  (2) \Leftrightarrow \frac{\partial S}{\partial \beta_1} &= 0 \\
  \Sigma_{i=1}^{n} w_ix_i(y_i - \mu_i) &= 0 \\
  \Sigma_{i=1}^{n} w_ix_i(y_i - \beta_0 - \beta_1 x_i) &= 0 \\
  \Sigma_{i=1}^{n} w_ix_i(y_i - \bar{y}_w + \beta_1 \bar{x}_w - \beta_1 x_i) &= 0 \\
  \beta_1 \Sigma_{i=1}^{n} w_ix_i(x_i - \bar{x}_w) &= \Sigma_{i=1}^{n} w_ix_i(y_i - \bar{y}_w) \\
  \beta_1 \left(\Sigma_{i=1}^{n} w_ix_i^2 - \frac{(\Sigma_{i=1}^{n} w_ix_i)^2}{\Sigma_{i=1}^{n}w_i}\right) &= \Sigma_{i=1}^{n}w_ix_iy_i - \Sigma_{i=1}^{n}w_ix_i\bar{y}_w \\
  \beta_1 \Sigma_{i=1}^{n}w_i(x - \bar{x}_w)^2 &= \Sigma_{i=1}^{n} w_i(x_i - \bar{x}_w)y_i
\end{align*} \\
  \beta_1 &= \frac{\Sigma_{i=1}^{n} w_i(x_i - \bar{x}_w)y_i}{\Sigma_{i=1}^{n}w_i(x - \bar{x}_w)^2}
$$

### 2.3
